Add wellfounded relation. compilation time TOO BIG

language_formalisation/type_system/declarational.v
@@ -1,73 +1,130 @@
-Add LoadPath "C:\Users\Ziga\Documents\Ziga_podatki\PHD\language_formalisation\syntax".
-Add LoadPath "C:\Users\Ziga\Documents\Ziga_podatki\PHD\language_formalisation\type_system".
-(* Add LoadPath "E:\Ziga_Podatki\faks\PHD\language_formalisation\syntax". *)
-(* Add LoadPath "E:\Ziga_Podatki\faks\PHD\language_formalisation\type_system". *)
+(* Add LoadPath "C:\Users\Ziga\Documents\Ziga_podatki\PHD\language_formalisation\syntax". *)
+(* Add LoadPath "C:\Users\Ziga\Documents\Ziga_podatki\PHD\language_formalisation\type_system". *)
+Add LoadPath "E:\Ziga_Podatki\faks\PHD\language_formalisation\syntax".
+Add LoadPath "E:\Ziga_Podatki\faks\PHD\language_formalisation\type_system".
 Require Import syntax syntax_lemmas.
 
-Inductive has_vtype : ctx -> val -> vtype -> Prop :=
-| TypeUnit Γ : has_vtype Γ Unit TyUnit 
-| TypeInt Γ n : has_vtype Γ (Int n) TyInt
+Inductive wf_vtype : vtype -> Prop :=
+| WfUnit : wf_vtype TyUnit 
+| WfInt : wf_vtype TyInt
+| WfΣ A B: wf_vtype A -> wf_vtype B -> wf_vtype (TyΣ A B)
+| WfΠ A B : wf_vtype A -> wf_vtype B -> wf_vtype (TyΠ A B)
+| WfFun A C : wf_vtype A -> wf_ctype C -> wf_vtype (TyFun A C)
+| WfHandler C D : wf_ctype C -> wf_ctype D -> wf_vtype (TyHandler C D)
+
+with wf_ctype : ctype -> Prop :=
+| WfCty A Σ E : wf_vtype A -> wf_sig Σ -> wf_eqs E Σ -> wf_ctype (CTy A Σ E)
+    
+with wf_sig : sig -> Prop :=
+| WfSigØ : wf_sig SigØ
+| WfSigU Σ op Aop Bop: 
+    wf_sig Σ -> wf_vtype Aop -> wf_vtype Bop -> wf_sig (SigU Σ op Aop Bop)
+
+with wf_ctx : ctx -> Prop :=
+| WfCtxØ : wf_ctx CtxØ
+| WfCtxU Γ A : wf_ctx Γ -> wf_vtype A -> wf_ctx (CtxU Γ A)
+
+with wf_tctx : tctx -> Prop :=
+| WfTCtxØ : wf_tctx TCtxØ
+| WfTCtxU Γ A : wf_tctx Γ -> wf_vtype A -> wf_tctx (TCtxU Γ A)
+
+with wf_tmpl : ctx -> tctx -> tmpl -> sig -> Prop :=
+| WfTApp Γ Z name num v A Σ : 
+    has_vtype Γ v A -> get_ttype Z num = Some A ->
+    wf_tmpl Γ Z (TApp (name, num) v) Σ
+| WfΠTMatch Γ Z v A B x y T Σ :
+    has_vtype Γ v (TyΠ A B) -> wf_tmpl (CtxU (CtxU Γ A) B) Z T Σ -> 
+    wf_tmpl Γ Z (TΠMatch v x y T) Σ
+| WfΣTMatch Γ Z v x A Tl y B Tr Σ :
+    has_vtype Γ v (TyΣ A B) -> wf_tmpl (CtxU Γ A) Z Tl Σ -> 
+    wf_tmpl (CtxU Γ B) Z Tr Σ -> wf_tmpl Γ Z (TΣMatch v x Tl y Tr) Σ
+| WfTOp Γ Z op A_op B_op v y T Σ :
+    get_op_type Σ op = Some (A_op, B_op) -> has_vtype Γ v A_op ->
+    wf_tmpl (CtxU Γ B_op) Z T Σ -> wf_tmpl Γ Z (TOp op v y T) Σ
+
+with wf_eqs : eqs -> sig -> Prop :=
+| WfEqsØ Σ : wf_eqs EqsØ Σ
+| WfEqsU E Γ Z T1 T2 Σ: 
+    wf_eqs E Σ -> wf_tmpl Γ Z T1 Σ -> wf_tmpl Γ Z T1 Σ -> 
+    wf_eqs (EqsU E Γ Z T1 T2) Σ
+
+with has_vtype : ctx -> val -> vtype -> Prop :=
+| TypeV Γ v A : wf_ctx Γ ->  wf_vtype A -> has_vtype' Γ v A -> has_vtype Γ v A
+
+with has_vtype' : ctx -> val -> vtype -> Prop :=
+| TypeUnit Γ : has_vtype' Γ Unit TyUnit 
+| TypeInt Γ n : has_vtype' Γ (Int n) TyInt
 | TypeVar Γ name num A :
     get_vtype Γ num = Some A ->
-    has_vtype Γ (Var (name, num)) A
+    has_vtype' Γ (Var (name, num)) A
 | TypePair Γ v1 v2 A B :
     has_vtype Γ v1 A ->
     has_vtype Γ v2 B ->
-    has_vtype Γ (Pair v1 v2) (TyΠ A B)
+    has_vtype' Γ (Pair v1 v2) (TyΠ A B)
 | TypeInl Γ v A B :
     has_vtype Γ v A ->
-    has_vtype Γ (Inl v) (TyΣ A B)
+    has_vtype' Γ (Inl v) (TyΣ A B)
 | TypeInr Γ v A B :
     has_vtype Γ v B ->
-    has_vtype Γ (Inr v) (TyΣ A B)
+    has_vtype' Γ (Inr v) (TyΣ A B)
 | TypeFun Γ x c A C :
     has_ctype (CtxU Γ A) c C ->
-    has_vtype Γ (Fun x c) (TyFun A C)
-| TypeHandler Γ x c_ret h A sig eqs D :
+    has_vtype' Γ (Fun x c) (TyFun A C)
+| TypeHandler Γ x c_ret h A Σ E D :
     has_ctype (CtxU Γ A) c_ret D ->
-    has_htype Γ h sig D ->
-    has_vtype Γ (Handler x c_ret h) (TyHandler (CTy A sig eqs) D)
+    has_htype Γ h Σ D ->
+    has_vtype' Γ (Handler x c_ret h) (TyHandler (CTy A Σ E) D)
+
 with has_ctype : ctx -> comp -> ctype -> Prop :=
+| TypeC Γ c C : wf_ctx Γ -> wf_ctype C -> has_ctype' Γ c C -> has_ctype Γ c C
+
+with has_ctype' : ctx -> comp -> ctype -> Prop :=
 | TypeRet Γ v A : 
     has_vtype Γ v A ->
-    has_ctype Γ (Ret v) (CTy A SigØ EqsØ)
+    has_ctype' Γ (Ret v) (CTy A SigØ EqsØ)
 | TypeΠMatch Γ v A B x y c C :
     has_vtype Γ v (TyΠ A B) ->
     has_ctype (CtxU (CtxU Γ A) B) c C ->
-    has_ctype Γ (ΠMatch v (x, y) c) C
+    has_ctype' Γ (ΠMatch v (x, y) c) C
 | TypeΣMatch Γ v A B xl cl xr cr C :
     has_vtype Γ v (TyΣ A B) ->
     has_ctype (CtxU Γ A) cl C ->
     has_ctype (CtxU Γ B) cr C ->
-    has_ctype Γ (ΣMatch v xl cl xr cr) C
+    has_ctype' Γ (ΣMatch v xl cl xr cr) C
 | TypeDoBind Γ x c1 c2 A B Σ eqs :
     has_ctype Γ c1 (CTy A Σ eqs) ->
     has_ctype (CtxU Γ A) c2 (CTy B Σ eqs) ->
-    has_ctype Γ (DoBind x c1 c2) (CTy B Σ eqs)
+    has_ctype' Γ (DoBind x c1 c2) (CTy B Σ eqs)
 | TypeApp Γ v1 v2 A C :
     has_vtype Γ v1 (TyFun A C) ->
     has_vtype Γ v2 A ->
-    has_ctype Γ (App v1 v2) C
+    has_ctype' Γ (App v1 v2) C
 | TypeHandle Γ v c C D :
     has_vtype Γ v (TyHandler C D) ->
     has_ctype Γ c C ->
-    has_ctype Γ (Handle v c) D
+    has_ctype' Γ (Handle v c) D
 | TypeLetRec Γ f x A C c1 c2 D:
     has_ctype (CtxU (CtxU Γ A) (TyFun A C)) c1 C ->
     has_ctype (CtxU Γ (TyFun A C)) c2 D ->
-    has_ctype Γ (LetRec f x c1 c2) D
+    has_ctype' Γ (LetRec f x c1 c2) D
 | TypeOp Γ op_id v y c A_op B_op A Σ eqs :
     get_op_type Σ op_id = Some (A_op, B_op) ->
     has_vtype Γ v A_op ->
     has_ctype (CtxU Γ B_op) c (CTy A Σ eqs) ->
-    has_ctype Γ (Op op_id v y c) (CTy A Σ eqs)
+    has_ctype' Γ (Op op_id v y c) (CTy A Σ eqs)
+    
 with has_htype : ctx -> hcases -> sig -> ctype -> Prop :=
-| TypeCasesØ Γ D : has_htype Γ CasesØ SigØ D
+| TypeH Γ h Σ D : 
+    wf_ctx Γ -> wf_sig Σ -> wf_ctype D -> has_htype' Γ h Σ D -> 
+    has_htype Γ h Σ D
+
+with has_htype' : ctx -> hcases -> sig -> ctype -> Prop :=
+| TypeCasesØ Γ D : has_htype' Γ CasesØ SigØ D
 | TypeCasesU Γ h op_id x k c_op A_op B_op Σ D :
     find_op_case h op_id = None ->
     has_htype Γ h Σ D ->
     has_ctype (CtxU (CtxU Γ (TyFun B_op D)) A_op) c_op D ->
-    has_htype 
+    has_htype' 
       Γ (CasesU h op_id x k c_op)
       (SigU Σ op_id A_op B_op) D
 .
