language_formalisation/type_system/type_aux_lemmas.v
@@ -1,12 +1,12 @@
-Add LoadPath "C:\Users\Ziga\Documents\Ziga_podatki\PHD\language_formalisation\syntax".
-Add LoadPath "C:\Users\Ziga\Documents\Ziga_podatki\PHD\language_formalisation\type_system".
-Add LoadPath "C:\Users\Ziga\Documents\Ziga_podatki\PHD\language_formalisation\substitution".
-(* Add LoadPath "E:\Ziga_Podatki\faks\PHD\language_formalisation\syntax". *)
-(* Add LoadPath "E:\Ziga_Podatki\faks\PHD\language_formalisation\type_system". *)
-(* Add LoadPath "E:\Ziga_Podatki\faks\PHD\language_formalisation\substitution". *)
+(* Add LoadPath "C:\Users\Ziga\Documents\Ziga_podatki\PHD\language_formalisation\syntax". *)
+(* Add LoadPath "C:\Users\Ziga\Documents\Ziga_podatki\PHD\language_formalisation\type_system". *)
+(* Add LoadPath "C:\Users\Ziga\Documents\Ziga_podatki\PHD\language_formalisation\substitution". *)
+Add LoadPath "E:\Ziga_Podatki\faks\PHD\language_formalisation\syntax".
+Add LoadPath "E:\Ziga_Podatki\faks\PHD\language_formalisation\type_system".
+Add LoadPath "E:\Ziga_Podatki\faks\PHD\language_formalisation\substitution".
 
 Require Export syntax syntax_lemmas declarational substitution Omega Logic.
-Require Export subs_lemmas.
+Require Export subs_lemmas wellfounded_lemmas.
 
 Ltac inv H := inversion H; clear H; subst.
 
@@ -16,22 +16,23 @@ Lemma extend_get_proof Γ A i Ai:
 Proof.
 assert (i + 1 = S i) by omega.
 induction Γ; rewrite H; auto.
-Qed.
+Defined.
 
 
 Fixpoint v_insert_typesafe Γ v A A_ins i {struct v} :
-  has_vtype Γ v A ->
+  has_vtype Γ v A -> wf_vtype A_ins ->
   has_vtype (ctx_insert_var Γ A_ins i) (Sub.v_shift v 1 i) A
 with c_insert_typesafe Γ c C A_ins i {struct c} :
-  has_ctype Γ c C ->
+  has_ctype Γ c C -> wf_vtype A_ins ->
   has_ctype (ctx_insert_var Γ A_ins i) (Sub.c_shift c 1 i) C
 with h_insert_typesafe Γ h Σ D A_ins i {struct h} :
-  has_htype Γ h Σ D ->
+  has_htype Γ h Σ D -> wf_vtype A_ins ->
   has_htype (ctx_insert_var Γ A_ins i) (Sub.h_shift h 1 i) Σ D.
 Proof.
 {
 clear v_insert_typesafe.
-revert A i. induction v; intros A i orig; simpl; inv orig.
+revert A i. induction v; intros A i orig wf_Ains; simpl; 
+inv orig; inv H1; apply TypeV; try (assumption || apply ctx_insert_wf; assumption).
 + simpl. assert (
     (if i <=? num then (name, num + 1) else (name, num))
       = (name, if i <=? num then num + 1 else num) ) 
@@ -46,76 +47,81 @@ revert A i. induction v; intros A i orig; simpl; inv orig.
     * apply leb_iff_conv in cmp. omega.
 + apply TypeUnit.
 + apply TypeInt.
-+ apply TypeInl. apply IHv. assumption.
-+ apply TypeInr. apply IHv. assumption.
++ apply TypeInl. apply IHv; assumption.
++ apply TypeInr. apply IHv; assumption.
 + apply TypePair; try apply IHv1 || apply IHv2; assumption.
 + apply TypeFun. rewrite ctx_insert_extend. auto.
 + apply TypeHandler; auto. rewrite ctx_insert_extend. auto.
 }{
 clear c_insert_typesafe.
-revert Γ C i. induction c; intros Γ C i orig; simpl; inv orig.
-+ apply TypeRet. auto.
+revert Γ C i. induction c; intros Γ C i orig wfAins; simpl;
+inv orig; inv H1; apply TypeC; try (assumption || apply ctx_insert_wf; assumption).
++ apply TypeRet. apply v_insert_typesafe; assumption.
 + eapply TypeΠMatch.
-  - eapply v_insert_typesafe. exact H4.
+  - eapply v_insert_typesafe. exact H7. assumption.
   - rewrite ctx_insert_extend. rewrite ctx_insert_extend.
-    assert (i+1+1=i+2) by omega. rewrite H. auto.
+    assert (i+1+1=i+2) by omega. rewrite H1. auto.
 + eapply TypeΣMatch.
-  - apply v_insert_typesafe. exact H6.
+  - apply v_insert_typesafe. exact H9. assumption.
   - rewrite ctx_insert_extend. auto.
   - rewrite ctx_insert_extend. auto.
 + eapply TypeApp.
-  - apply v_insert_typesafe. exact H2.
+  - apply v_insert_typesafe. exact H5. assumption.
   - auto.
-+ eapply TypeOp. exact H5. auto.
++ eapply TypeOp. exact H8. auto.
   rewrite ctx_insert_extend. auto.
 + eapply TypeLetRec.
   - rewrite ctx_insert_extend. rewrite ctx_insert_extend.
-    assert (i+1+1=i+2) by omega. rewrite H. apply IHc1. exact H5.
+    assert (i+1+1=i+2) by omega. rewrite H1. apply IHc1. exact H8. assumption.
   - rewrite ctx_insert_extend. auto.
 + eapply TypeDoBind.
-  - apply IHc1. exact H4.
+  - apply IHc1. exact H7. assumption.
   - rewrite ctx_insert_extend. auto.
 + eapply TypeHandle.
-  - apply v_insert_typesafe. exact H2.
+  - apply v_insert_typesafe. exact H5. assumption.
   - auto.
 }{
 clear h_insert_typesafe.
-revert Γ Σ D i. induction h; intros Γ Σ D i orig; simpl; inv orig.
+revert Γ Σ D i. induction h; intros Γ Σ D i orig wf_Ains; simpl; 
+inv orig; inv H0; inv H1; apply TypeH; try (apply ctx_insert_wf; assumption); 
+try apply WfSigØ || apply WfCty || apply WfSigU; try assumption.
 + apply TypeCasesØ.
-+ apply TypeCasesU; auto.
++ inv H2.
++ inv H2.
++ inv H2. apply TypeCasesU; auto.
   - assert (forall h,
-      find_op_case h o = None ->
-      find_op_case (Sub.h_shift h 1 i) o = None).
+      find_op_case h op = None ->
+      find_op_case (Sub.h_shift h 1 i) op = None).
     * intros h' orig. induction h'; auto.
-      simpl in *. destruct (o==o0). discriminate. auto.
-    * apply H. assumption.
+      simpl in *. destruct (op==o). discriminate. auto.
+    * apply H1. assumption.
   - rewrite ctx_insert_extend. rewrite ctx_insert_extend.
-    assert (i+1+1=i+2) by omega. rewrite H. auto.
+    assert (i+1+1=i+2) by omega. rewrite H1. auto.
 }
-Qed.
+Defined.
 
 Fixpoint v_shift_typesafe
   (Γ:ctx) (A0:vtype) v A {struct v} :
-  has_vtype Γ v A ->
+  has_vtype Γ v A -> wf_vtype A0 ->
   has_vtype (CtxU Γ A0) (Sub.v_shift v 1 0) A
 
 with c_shift_typesafe
   (Γ:ctx) (A0:vtype) c C {struct c} :
-  has_ctype Γ c C ->
+  has_ctype Γ c C -> wf_vtype A0 ->
   has_ctype (CtxU Γ A0) (Sub.c_shift c 1 0) C
 
 with h_shift_typesafe
   (Γ:ctx) (A0:vtype) h Σ D {struct h} :
-  has_htype Γ h Σ D ->
+  has_htype Γ h Σ D -> wf_vtype A0 ->
   has_htype (CtxU Γ A0) (Sub.h_shift h 1 0) Σ D.
 Proof.
 all: intro orig;
 assert (ctx_insert_var Γ A0 0 = CtxU Γ A0) by (destruct Γ; auto);
-rewrite <-H.
-apply v_insert_typesafe. assumption.
-apply c_insert_typesafe. assumption.
-apply h_insert_typesafe. assumption.
-Qed.
+rewrite <-H; inv orig.
+apply v_insert_typesafe. apply TypeV; assumption.
+apply c_insert_typesafe. apply TypeC; assumption.
+apply h_insert_typesafe. apply TypeH; assumption.
+Defined.
 
 
 Fixpoint v_negshift_typesafe
@@ -138,8 +144,9 @@ with h_negshift_typesafe
 Proof.
 {
 clear v_negshift_typesafe.
-revert Γ A i. induction v; intros Γ A i orig no_var; simpl; inv orig;
-simpl in no_var.
+revert Γ A i. induction v; intros Γ A i orig no_var; simpl; 
+inv orig; inv H1; apply TypeV; simpl in no_var; 
+try (apply ctx_remove_wf; assumption); try assumption.
 + simpl. assert (
     (if i <=? num then (name, num - 1) else (name, num))
       = (name, if i <=? num then num - 1 else num) ) 
@@ -147,17 +154,17 @@ simpl in no_var.
   rewrite same. apply TypeVar. destruct (i<=?num) eqn:cmp.
   - erewrite <-get_ctx_remove_changed; apply leb_complete in cmp.
     * destruct num. destruct no_var. omega.
-      simpl. assert (num-0=num) by omega. rewrite H. assumption.
+      simpl. assert (num-0=num) by omega. rewrite H1. assumption.
     * omega.
   - erewrite <-get_ctx_remove_unchanged. assumption.
     apply leb_iff_conv in cmp. omega.
 + apply TypeUnit.
 + apply TypeInt.
-+ apply TypeInl. eapply IHv. exact H1. assumption.
-+ apply TypeInr. eapply IHv. exact H1. assumption.
++ apply TypeInl. eapply IHv. exact H4. assumption.
++ apply TypeInr. eapply IHv. exact H4. assumption.
 + apply TypePair; destruct no_var.
-  - eapply IHv1. exact H2. assumption.
-  - eapply IHv2. exact H4. assumption.
+  - eapply IHv1. exact H5. assumption.
+  - eapply IHv2. exact H7. assumption.
 + apply TypeFun. rewrite ctx_remove_extend.
   apply c_negshift_typesafe; assumption.
 + apply TypeHandler; destruct no_var.
@@ -165,49 +172,53 @@ simpl in no_var.
   - apply h_negshift_typesafe; assumption.
 }{
 clear c_negshift_typesafe.
-revert Γ C i. induction c; intros Γ C i orig no_var; simpl; inv orig;
-simpl in no_var; try destruct no_var.
+revert Γ C i. induction c; intros Γ C i orig no_var; inv orig; inv H1; inv H0;
+simpl in no_var; try destruct no_var; apply TypeC; simpl; 
+try (apply ctx_remove_wf; assumption); try (apply WfCty; assumption).
 + apply TypeRet. apply v_negshift_typesafe; assumption.
 + eapply TypeΠMatch.
-  - apply v_negshift_typesafe. exact H4. assumption.
+  - apply v_negshift_typesafe. exact H7. assumption.
   - rewrite ctx_remove_extend. rewrite ctx_remove_extend.
-    assert (i+1+1=i+2) by omega. rewrite H1. apply IHc; assumption.
-+ eapply TypeΣMatch; destruct H0.
-  - apply v_negshift_typesafe. exact H6. assumption.
+    assert (i+1+1=i+2) by omega. rewrite H5. apply IHc; assumption.
++ eapply TypeΣMatch; destruct H4.
+  - apply v_negshift_typesafe. exact H9. assumption.
   - rewrite ctx_remove_extend. apply IHc1; assumption.
   - rewrite ctx_remove_extend. apply IHc2; assumption.
 + eapply TypeApp; apply v_negshift_typesafe.
-  exact H2. all: assumption.
-+ eapply TypeOp. exact H5.
+  exact H5. all: assumption.
++ eapply TypeOp. exact H8.
   - apply v_negshift_typesafe; assumption.
   - rewrite ctx_remove_extend. apply IHc; assumption.
 + eapply TypeLetRec.
   - rewrite ctx_remove_extend. rewrite ctx_remove_extend.
-    assert (i+1+1=i+2) by omega. rewrite H1. apply IHc1. exact H5. assumption.
+    assert (i+1+1=i+2) by omega. rewrite H5. apply IHc1. exact H8. assumption.
   - rewrite ctx_remove_extend. apply IHc2; assumption.
 + eapply TypeDoBind.
-  - apply IHc1. exact H4. assumption.
+  - apply IHc1. exact H7. assumption.
   - rewrite ctx_remove_extend. auto.
 + eapply TypeHandle.
-  - apply v_negshift_typesafe. exact H2. assumption.
+  - apply v_negshift_typesafe. exact H5. assumption.
   - apply IHc; assumption.
 }{
 clear h_negshift_typesafe.
-revert Γ Σ i. induction h; intros Γ Σ i orig no_var; simpl; inv orig;
-simpl in no_var; try destruct no_var.
+revert Γ Σ i. induction h; intros Γ Σ i orig no_var; inv orig; inv H0; inv H2;
+inv H1; apply TypeH; auto; simpl in no_var; try destruct no_var;
+try (apply ctx_remove_wf; assumption); try (apply WfCty; assumption).
+- apply WfSigØ.
 - apply TypeCasesØ.
+- apply WfSigU; assumption.
 - apply TypeCasesU.
-  assert (forall h, find_op_case h o = None 
-    -> find_op_case (Sub.h_negshift h 1 i) o = None).
+  assert (forall h, find_op_case h op = None 
+    -> find_op_case (Sub.h_negshift h 1 i) op = None).
   + intro h'. induction h'; intro orig; auto.
-    simpl. simpl in orig. destruct (o==o0); auto. discriminate.
-  + apply H1. assumption.
+    simpl. simpl in orig. destruct (op==o); auto. discriminate.
+  + apply H8. assumption.
   + auto.
   + rewrite ctx_remove_extend. rewrite ctx_remove_extend.
-    assert (i+1+1=i+2) by omega. rewrite H1.
+    assert (i+1+1=i+2) by omega. rewrite H8.
     apply c_negshift_typesafe; assumption.
 }
-Qed.
+Defined.
 
 
 Fixpoint v_subs_typesafe
@@ -229,11 +240,11 @@ Proof.
 {
 clear v_subs_typesafe.
 revert Γ A i. induction v; intros Γ A i orig in_ctx vstyped;
-simpl; inv orig.
+simpl; inv orig; inv H1; apply TypeV; auto.
 + simpl in *. destruct (num=?i) eqn:cmp.
   * apply Nat.eqb_eq in cmp. rewrite <-cmp in in_ctx.
-    rewrite H1 in in_ctx. injection in_ctx. intro samety.
-    rewrite samety. assumption.
+    rewrite H4 in in_ctx. injection in_ctx. intro samety.
+    rewrite samety. inv vstyped. assumption.
   * apply TypeVar. assumption.
 + apply TypeUnit.
 + apply TypeInt.
@@ -242,14 +253,14 @@ simpl; inv orig.
 + apply TypePair; try apply IHv1 || apply IHv2; auto.
 + apply TypeFun. eapply c_subs_typesafe.
   - assumption.
-  - assert (i+1=S i) by omega. rewrite H. simpl.
+  - assert (i+1=S i) by omega. rewrite H1. simpl.
     exact in_ctx.
-  - apply v_shift_typesafe. assumption.
+  - apply v_shift_typesafe. assumption. inv H0. assumption.
 + apply TypeHandler.
   - eapply c_subs_typesafe.
     * assumption.
-    * assert (i+1=S i) by omega. rewrite H. simpl. exact in_ctx.
-    * apply v_shift_typesafe. assumption.
+    * assert (i+1=S i) by omega. rewrite H1. simpl. exact in_ctx.
+    * apply v_shift_typesafe. assumption. inv H0. inv H3. assumption.
   - eapply h_subs_typesafe.
     * assumption.
     * exact in_ctx.
@@ -259,49 +270,55 @@ clear c_subs_typesafe.
 assert (forall i, i+1=S i) as Si by (intro; omega).
 assert (forall i, i+2=S(S i)) as SSi by (intro; omega).
 revert Γ C i v_s. induction c; intros Γ C i v_s orig in_ctx vstyped;
-simpl; inv orig.
+simpl; inv orig; inv H1; apply TypeC; auto.
 + apply TypeRet. eapply v_subs_typesafe. 2 : exact in_ctx. all: assumption.
 + eapply TypeΠMatch.
-  - eapply v_subs_typesafe. exact H4. exact in_ctx. assumption.
+  - eapply v_subs_typesafe. exact H7. exact in_ctx. assumption.
   - apply IHc. assumption.
     * rewrite SSi. assumption.
     * rewrite <-(v_shift_shift 1 1 0).
       apply v_shift_typesafe. apply v_shift_typesafe. assumption.
+      all: (inv H7; inv H2; assumption).
 + eapply TypeΣMatch.
-  { eapply v_subs_typesafe. exact H6. exact in_ctx. assumption. }
+  { eapply v_subs_typesafe. exact H9. exact in_ctx. assumption. }
   all: try apply IHc1 || apply IHc2; try apply v_shift_typesafe; auto.
-  all: rewrite Si; assumption.
+  all: try (rewrite Si; assumption).
+  all: inv H9; inv H2; assumption.
 + eapply TypeApp.
-  - eapply v_subs_typesafe. exact H2. exact in_ctx. assumption.
+  - eapply v_subs_typesafe. exact H5. exact in_ctx. assumption.
   - eapply v_subs_typesafe. auto. exact in_ctx. assumption.
-+ eapply TypeOp. exact H5.
++ eapply TypeOp. exact H8.
   - eapply v_subs_typesafe. 2: exact in_ctx. assumption. assumption.
   - apply IHc; auto.
     * rewrite Si. assumption.
-    * apply v_shift_typesafe. assumption.
+    * apply v_shift_typesafe. assumption. inv H0.
+      eapply get_op_type_wf. exact H5. exact H8.
 + eapply TypeLetRec.
-  - apply IHc1. exact H5.
+  - apply IHc1. exact H8.
     * rewrite SSi. assumption.
     * rewrite <-(v_shift_shift 1 1 0).
       apply v_shift_typesafe. apply v_shift_typesafe. assumption.
+      ++ inv H9. inv H1. inv H7. assumption.
+      ++ inv H9. inv H1. assumption.
   - apply IHc2. assumption.
     * rewrite Si. assumption.
     * apply v_shift_typesafe. assumption.
+      inv H9. inv H1. assumption.
 + eapply TypeDoBind.
-  - apply IHc1. exact H4. assumption. assumption.
+  - apply IHc1. exact H7. assumption. assumption.
   - apply IHc2.
     * assumption.
     * rewrite Si. assumption.
-    * apply v_shift_typesafe. assumption.
+    * apply v_shift_typesafe. assumption. inv H7. inv H2. assumption.
 + eapply TypeHandle.
-  - eapply v_subs_typesafe. exact H2. exact in_ctx. assumption.
+  - eapply v_subs_typesafe. exact H5. exact in_ctx. assumption.
   - apply IHc; auto.
 }{
 clear h_subs_typesafe.
 assert (forall i, i+1=S i) as Si by (intro; omega).
 assert (forall i, i+2=S(S i)) as SSi by (intro; omega).
 revert Γ Σ D i v_s. induction h; intros Γ Σ D i v_s orig in_ctx vstyped;
-simpl; inv orig.
+simpl; inv orig; inv H2; apply TypeH; auto.
 + apply TypeCasesØ.
 + apply TypeCasesU.
   assert (forall h,
@@ -310,24 +327,25 @@ simpl; inv orig.
   * intros h' cantfind. induction h'. auto.
     simpl. simpl in cantfind. destruct (o==o0). discriminate.
     apply IHh'. exact cantfind.
-  * apply H. assumption.
+  * apply H2. assumption.
   * auto.
   * rewrite SSi. eapply c_subs_typesafe; auto.
     - simpl. exact in_ctx.
     - rewrite <-(v_shift_shift 1 1 0).
       apply v_shift_typesafe. apply v_shift_typesafe. assumption.
 }
-Qed.
+Defined.
 
 Lemma h_has_case Γ h Σ D op A_op B_op:
   has_htype Γ h Σ D ->
   get_op_type Σ op = Some (A_op, B_op) ->
   exists x k c_op, find_op_case h op = Some (x, k, c_op).
 Proof.
-revert Γ Σ. induction h; intros Γ Σ typed gets.
-+ inv typed. simpl in gets. discriminate.
-+ inv typed. simpl in *. destruct (op==o).
+revert Γ Σ. induction h; intros Γ Σ typed gets;
+inv typed; inv H1; inv H2.
++ simpl in gets. discriminate.
++ simpl in *. destruct (op==o).
   - injection gets. intros. subst.
     exists v. exists v0. exists c. reflexivity.
-  - apply IHh in H8; assumption.
-Qed.
+  - apply IHh in H14; assumption.
+Defined.
