language_formalisation/type_system/wellfounded_lemmas.v
@@ -1,0 +1,46 @@
+(* Add LoadPath "C:\Users\Ziga\Documents\Ziga_podatki\PHD\language_formalisation\syntax". *)
+(* Add LoadPath "C:\Users\Ziga\Documents\Ziga_podatki\PHD\language_formalisation\type_system". *)
+(* Add LoadPath "C:\Users\Ziga\Documents\Ziga_podatki\PHD\language_formalisation\substitution". *)
+Add LoadPath "E:\Ziga_Podatki\faks\PHD\language_formalisation\syntax".
+Add LoadPath "E:\Ziga_Podatki\faks\PHD\language_formalisation\type_system".
+Add LoadPath "E:\Ziga_Podatki\faks\PHD\language_formalisation\substitution".
+
+Require Export syntax syntax_lemmas declarational substitution Omega Logic.
+Require Export subs_lemmas.
+
+Lemma ctx_insert_wf Γ A i:
+  wf_ctx Γ -> wf_vtype A -> wf_ctx (ctx_insert_var Γ A i).
+Proof.
+revert i A; induction Γ; intros i A orig wfv.
++ induction i; simpl.
+  * apply WfCtxU; assumption.
+  * apply WfCtxØ.
++ induction i; simpl.
+  * apply WfCtxU; assumption.
+  * inv orig. apply WfCtxU; try apply IHΓ; assumption.
+Defined.
+
+Lemma ctx_remove_wf Γ i:
+  wf_ctx Γ -> wf_ctx (ctx_remove_var Γ i).
+Proof.
+revert i; induction Γ; intros i orig.
++ induction i; simpl; apply WfCtxØ.
++ induction i; simpl; inv orig.
+  * assumption.
+  * apply WfCtxU; try apply IHΓ; assumption.
+Defined.
+
+Lemma get_op_type_wf Σ op A_op B_op:
+  wf_sig Σ -> get_op_type Σ op = Some (A_op, B_op) ->
+  wf_vtype A_op /\ wf_vtype B_op.
+Proof.
+induction Σ; intros orig gets; constructor.
++ simpl in gets. discriminate.
++ simpl in gets. discriminate.
++ simpl in *. destruct (op == o).
+  - injection gets. intros. subst. inv orig. assumption.
+  - inv orig. apply IHΣ; assumption.
++ simpl in *. destruct (op == o).
+  - injection gets. intros. subst. inv orig. assumption.
+  - inv orig. apply IHΣ; assumption.
+Defined.
